\title{}
\author{
  \textsc{Jeff Wendling}
}
\date{\today}
\documentclass[11pt]{article}
\usepackage{amsfonts,amsmath,amssymb,amsbsy,amsthm}
\usepackage{latexsym,bm}
\usepackage{upgreek}
\usepackage{graphics,graphicx}
\usepackage{subfigure}
\usepackage{subfigmat}
\usepackage{psfrag}
\usepackage{url}
\usepackage[square,numbers,comma,sort&compress]{natbib}
\usepackage{float}

%macro for unnumbered aligned environments
\newcommand{\eq}[1]{\begin{align*}#1\end{align*}}

%macro for numbered equations
\newcommand{\eqn}[2]{
  \begin{equation}
    \label{#1}
    #2
  \end{equation}
}

%macro for referencing equations
\newcommand{\eqr}[1]{eqn~(\ref{#1})}

%macro for frac partials
\newcommand{\fp}[2]{\frac{\partial#1}{\partial#2}}
\newcommand{\fpp}[2]{\frac{\partial^2 #1}{\partial#2^2}}

%macro for inline partials
\newcommand{\p}[1]{\partial_{#1}}

\begin{document}
\begin{center}
{\large\bf 
Jeff Wendling\\
\today\\
Math 528: Elementary Fluid Dynamics I\\
Homework \#5
}
\end{center}
\begin{description}
\item[8.1] Rewrite the exact 2-D equations of motion in terms of the non-dimensional
and scaled variables
$$
  x' = \frac{x}{L},
  \qquad
  y' = \frac{y}{R^{-\frac{1}{2}}L},
  \qquad
  u' = \frac{u}{U_0},
  \qquad
  v' = \frac{v}{R^{-\frac{1}{2}}L},
  \qquad
  p' = \frac{p}{\rho U_0^2},
$$
where $R = U_0L/\nu$. By taking the limit $R \rightarrow \infty$
\emph{with fixed $u'$, $\partial u' / \partial x'$}, etc., derive the boundary
layer equations in their non-dimensional and scaled form:
$$
  u' \fp{u'}{x'} + v'\fp{u'}{y'} = -\fp{p'}{x'} + \fpp{u'}{y'},
$$
$$
  0 = -\fp{p'}{y'},
  \qquad
  \fp{u'}{x'} + \fp{v'}{y'} = 0.
$$
\item[Solution] We begin by calculating
\begin{align}
\label{relations}
\nonumber  \fp{u'}{x'} &= \frac{L}{U_0} \fp{u}{x} &
           \fp{v'}{x'} &= \frac{L\sqrt{R}}{U_0} \fp{v}{x} \\
\nonumber  \fp{u'}{y'} &= \frac{L}{\sqrt{R}U_0} \fp{u}{y} &
           \fp{v'}{y'} &= \frac{L}{U_0} \fp{v}{y} \\
\nonumber  \fp{p'}{x'} &= \frac{L}{\rho U_0^2} \fp{p}{x} &
           \fp{p'}{y'} &= \frac{L}{\rho U_0^2 \sqrt{R}} \fp{p}{y} \\
\nonumber  \fpp{u'}{(x')} &= \frac{L^2}{U_0} \fpp{u}{x} &
           \fpp{v'}{(x')} &= \frac{L^2\sqrt{R}}{U_0} \fpp{v}{x} \\
           \fpp{u'}{(y')} &= \frac{L^2}{RU_0} \fpp{u}{y} &
           \fpp{v'}{(y')} &= \frac{L^2}{\sqrt{R}U_0} \fpp{v}{y}
\end{align}
Substituting \eqr{relations} into the first part of the equations of motion,
$$
  u \fp{u}{x} + v \fp{u}{y} = -\frac{1}{\rho} \fp{p}{x} + \nu \fpp{u}{x} + \nu \fpp{u}{y}
$$
we obtain
\eq{
  u' \frac{U_0^2}{L} \fp{u'}{x'}
  + v' \frac{U_0^2}{L} \fp{u'}{y'}
  &= 
  -\frac{U_0^2}{L} \fp{p'}{x'}
  + \frac{\nu U_0}{L^2} \fpp{u'}{(x')}
  + \frac{\nu U_0 R}{L^2} \fpp{u'}{(y')}
  \\
%
%
  \frac{U_0^2}{L}\bigg(
  u' \fp{u'}{x'}
  + v' \fp{u'}{y'}
  &=
  - \fp{p'}{x'}
  + \frac{\nu}{U_0 L} \fpp{u'}{(x')}
  + \frac{\nu R}{U_0 L} \fpp{u'}{(y')}
  \bigg)
}
But because $R^{-1} = \frac{\nu}{U_0 L}$, we have that as $R \rightarrow \infty$
$$
  u' \fp{u'}{x'}
  + v' \fp{u'}{y'}
  =
  - \fp{p'}{x'}
  + \fpp{u'}{(y')}
$$
Substitutiong \eqr{relations} into the second part of the equations of motion,
$$
  u \fp{v}{x} + v \fp{v}{y} = -\frac{1}{\rho} \fp{p}{y} + \nu \fpp{v}{x} + \nu \fpp{v}{y}
$$
we obtain
\eq{
  u' \frac{U_0^2}{L\sqrt{R}} \fp{v'}{x'}
  + v' \frac{U_0^2}{L\sqrt{R}} \fp{v'}{y'}
  &=
  -\frac{U_0^2 \sqrt{R}}{L} \fp{p'}{y'}
  + \frac{\nu U_0}{L^2 \sqrt{R}} \fpp{v'}{(x')}
  + \frac{\nu U_0 \sqrt{R}}{L^2} \fpp{v'}{(y')}
  \\
%
%
  \frac{\sqrt{R}U_0^2}{L}\bigg(
  u' \frac{1}{R} \fp{v'}{x'}
  + v' \frac{1}{R} \fp{v'}{y'}
  &=
  -\fp{p'}{y'}
  + \frac{1}{R^2} \fpp{v'}{(x')}
  + \frac{1}{R} \fpp{v'}{(y')}
  \bigg)
}
which as $R \rightarrow \infty$ yields
$$
  0
  =
  - \fp{p'}{y'}
$$
Substituting \eqr{relations} into the third part of the equations of motion,
$$
  \fp{u}{x} + \fp{v}{y} = 0
$$
we obtain,
\eq{
    \frac{U_0}{L} \fp{u'}{x'} &+ \frac{U_0}{L} \fp{v'}{y'} = 0\\
    \fp{u'}{x'} &+ \fp{v'}{y'} = 0
}
%
\hfill $\blacksquare$
\item[8.2] Consider the boundary layer near the forward stagnation point on some
2-D body, such as a circular cylinder (see Fig.~8.14). The mainstream flow at the
edge of the boundary layer is $U(x) = \alpha x$, where $x$ denotes the distance
along the boundary measured from the stagnation point and $\alpha$ is a postive
constant (see eqn (4.23)). Seek a similarity solution of the boundary layer
equations in which
$$
  u(x, y) = \alpha x f'(\eta),
  \qquad
  \text{where} \; \eta = y / g(x)
$$
and deduce that g(x) must be a constant. By choosing that constant as
$(\nu/\alpha)^{\frac{1}{2}}$ show that the problem can be reduced to
$$
  f''' + ff'' + 1 - f'^2 = 0
$$
subject to
$$
  f(0) = f'(0) = 0,
  \qquad
  f'(\infty) = 1.
$$
\item[Solution]
Given that $u(x,y) = \alpha x f'(\eta)$ with $\eta = y/g(x)$, and $U = \alpha x$,
we calculate
\begin{align}
\label{relations82}
\nonumber  \p{x}u &= \alpha f'(\eta) - \alpha xf''(\eta)y g^{-2}(x)g'(x) \\
\nonumber  \p{y}u &= \alpha x f''(\eta) g^{-1}(x) \\
           \fpp{u}{y} &= \alpha x f'''(\eta) g^{-2}(x)
\end{align}
Substituting the relations in \eqr{relations82} into the equations of motion
on the boundary,
$$
  u \fp{u}{x} + v\fp{u}{y} = UU' + \nu\fpp{u}{y}
$$
yielding the equation
\begin{align}
\label{similarity}
\nonumber
  \alpha x f'
  \left(\alpha f' - \alpha x f''yg^{-2}g'\right)
  + v\left(\alpha x f'' g^{-1} \right)
  &=
  \alpha^2 x
  + \nu \left(\alpha x f''' g^{-2} \right)
  \\
%
%
  \alpha^2 x g^2 f'^2
  - \alpha^2 x^2 f'f''yg'
  + vg \alpha x f''
  &=
  \alpha^2 x g^2
  + \nu \alpha x f'''
\end{align}
which we notice that the only way for this to become and ODE in $f$ is if
$g' = 0$ so that the second term drops out. Thus, $g$ is a constant. This reduces
\eqr{similarity} to
\eqn{similarity_reduce}{
  \alpha g^2 f'^2
  + vg f''
  =
  \alpha g^2
  + \nu f'''
}
We choose $g = \sqrt{\dfrac{\nu}{\alpha}}$. Because $g$ is a constant, we can
write
$$
  \p{y}v = -\p{x}u = -\alpha f'(\eta)
$$
so
\eqn{v_solution}{
  v = -\sqrt{\nu\alpha}f + k(x)
}
Plugging \eqr{v_solution} and our choice for $g$ into \eqr{similarity_reduce} yields
\eqn{almost_soln}{
  \nu f'^2
  - \nu f f''
  + k gf''
  =
  \nu
  + \nu f'''
}
Choosing our constant of integration $k(x) = 0$ and dividing through by $\nu$
in \eqr{almost_soln} gives the ode
$$
  f''' + ff'' + 1 - f'^2 = 0
$$
We apply the no slip conditions,
$$
  f(0) = f'(0) = 0
$$
which means that $u(x, 0) = 0$ where $y$ is the normal distance from the boundary.
We also require the matching condition
$$
  f'(\infty) = 1
$$
which makes $u = U$ outside the boundary layer.
%
\hfill $\blacksquare$
\item[8.3] Consider a general similarity solution
$$
  \psi = F(x)f(\eta),
  \qquad
  \eta = y / g(x)
$$
to the boundary layer equations (8.1) and (8.2), where $\psi$ denotes the stream
function. Show that the mainstream condition (8.9) demands that
$F(x) = cU(x)g(x)$, where $c$ is a constant, and then, for convenience, choose
$c$ to be 1. Show that substitution in the boundary layer equations leads to
$$
  f'^2
  - \left(1 + \frac{U}{U'}\frac{g'}{g}\right)ff''
  =
  1 
  + \frac{\nu f'''}{g^2 U'}
  ,
$$
where a prime denotes differentiation with respect to the appropriate single 
variable in each case. Deduce that a similarity solution is only possible if
$$
  \text{\emph{either}}
  \qquad
  U(x) \propto (x - x_0)^m
  \qquad
  \text{\emph{or}}
  \qquad
  U(x) \propto e^{\alpha x}
$$
where $x_0$, $m$, and $\alpha$ are constants.

In the case
$$
  U(x) = Ax^m,
  \qquad
  A > 0,
$$
show that g(x) is proportional to $x^{\frac{1}{2}(1-m)}$, and show that choosing
$$
  g(x)
  =
  \bigg[
  \frac{2\nu}{(m+1)Ax^{m-1}}
  \bigg]^{\frac{1}{2}}
$$
leads to
$$
  f''' + ff'' + \frac{2m}{m+1}(1-f'^2) = 0,
$$
subject to
$$
  f(0) = f'(0) = 0,
  \qquad
  f'(\infty) = 1.
$$
Verify that flow past a plate (\S 8.3) and flow near a foward stagnation point
(Exercise 8.2) are special cases of these \emph{Falker-Skan equations}.
\item[Solution]
We have from the stream function
$$
  u = \fp{\psi}{y} = \frac{F f'}{g}
$$
If we have $\eta \rightarrow \infty$, and call $f'(\infty) = \frac{1}{c}$, then
for the mainstream condition to hold we must have
$$
  U = \frac{F\frac{1}{c}}{g}
  \implies
  F = cgU
$$
To substitute into the boundary layer equations, we begin by calculating
\eq{
  u &= \frac{1}{g}\left( Ff' \right) \\
  v &= \frac{1}{g^2}\left(Ff'g'y - g^2F'f \right) \\
  \p{x}u &= \frac{1}{g^3}\left( g^2F'f' - yg'Ff'' - Ff'g'g \right) \\
  \p{y}u &= \frac{1}{g^2}\left( F f'' \right) \\
  \p{yy}u &= \frac{1}{g^3}\left( F f''' \right) \\
}
Now we substitute into the boundary layer equations,
$$
  u \fp{u}{x} + v\fp{u}{y} = UU' + \nu\fpp{u}{y}
$$
and obtain
\eq{
  \frac{FF'f'^2}{g}
  - \underbrace{
  \frac{yg'F^2f'f''}{g^3}
  + \frac{F^2f'g'yf''}{g^3}
  }_{=0}
  - \frac{F^2f'^2 g'}{g^2}
  - \frac{F'Fff''}{g}
  &=
  FU'
  + \frac{\nu Ff'''}{g^2}
  \\
%
%
  F\bigg(
  \frac{F'f'^2}{g}
  - \frac{Ff'^2 g'}{g^2}
  - \frac{F'ff''}{g}
  &=
  U'
  + \frac{\nu f'''}{g^2}
  \bigg)
  \\
%
%
  \frac{U'gf'^2}{g}
  + \underbrace{
  \frac{g'Uf'^2}{g}
  - \frac{Ugf'^2 g'}{g^2}
  }_{=0}
  - \frac{U'gff''}{g}
  - \frac{g'Uff''}{g}
  &=
  U'
  + \frac{\nu f'''}{g^2}
  \\
%
%
  U'\bigg(
  f'^2
  - \big(
  1
  + \frac{U}{U'}\frac{g'}{g}
  \big) ff''
  &=
  1
  + \frac{\nu f'''}{g^2U'}
  \bigg)
%
%
}
Thus,
\eqn{main_equation}{
  f'^2
  - \bigg(
  1
  + \frac{U}{U'}\frac{g'}{g}
  \bigg) ff''
  =
  1
  + \frac{\nu f'''}{g^2U'}
}

The only way \eqr{main_equation} can be an ODE in $f$ is if we have the conditions
$$
  \frac{U}{U'}\frac{g'}{g} = c,
  \qquad
  g^2 U' = d
$$
The first relation leads to
\begin{align}
\nonumber  \frac{U}{U'}\frac{g'}{g} &= c_1 \\
\nonumber  \frac{U'}{U} &= e \frac{g'}{g} \\
\nonumber  \ln U &= e\ln g + f \\
\label{u_relation}  U &= f g^e \\
\label{up_relation}  U' &= h g^{e-1} g'
\end{align}
Substituting \eqr{up_relation} into the second condition gives
\begin{align}
\nonumber  g^2 h g^{e-1} g' &= d \\
\label{g_soln} g^{e+1} g' &= i
\end{align}
Now, \eqr{g_soln} has two solutions depending on the constant $e+1$ given by,
\begin{align}
\label{g_soln_1} g &\propto (x - x_0)^m & e+1 \neq -1 \\
\label{g_soln_2} g &\propto e^{\alpha x} & e+1 = -1
\end{align}
Using \eqr{u_relation} we can see that either (abusing some notation with the consants)
$$
  U \propto (x - x_0)^m
  \qquad
  \text{\emph{or}}
  \qquad
  U \propto e^{\alpha x}
$$
If we assume that
\eqn{u_assump}{
  U = Ax^m
}
then we can easily see using $g^2 U' = d$ that
\begin{align}
\nonumber g^2 &\propto \frac{1}{U'} \\
\nonumber &\propto x^{1-m} \\
\label{g_propto} g &\propto x^{\frac{1}{2}(1-m)}
\end{align}
We choose
\eqn{g_assump}{
  g
  = 
  \bigg[
  \frac{2\nu}{(m+1)Ax^{m-1}}
  \bigg]^\frac{1}{2}
}
and attempt to substitute \eqr{u_assump} and \eqr{g_assump} into \eqr{main_equation}.
To this end, we calculate
\begin{align}
  \nonumber
  g^2 U'
  &=
  \frac{mAx^{m-1} 2\nu}{m+1 A x^{m-1}}
  \\
%
%
  \label{second_term}
  &=
  \frac{2m}{m+1}\nu
\end{align}
and
\begin{align}
  \nonumber
  1 + \frac{U}{U'}\frac{g'}{g} 
  &=
  1
  + \frac{Ax^m}{mAx^{m-1}}
  (-\frac{1}{2})
  \bigg[
  \frac{2\nu}{(m+1)Ax^{m-1}}
  \bigg]^{-1}
  \frac{2\nu(1-m)}{(m+1)A x^m}
  \\
%
%
  \nonumber
  &=
  1
  + \frac{x}{m}
  (-\frac{1}{2})
  \frac{(1-m)}{x}
  \\
%
%
  \label{first_term}
  &=
  1
  + \frac{m - 1}{2m}
  =
  \frac{m + 1}{2m}
\end{align}
We plug \eqr{second_term} and \eqr{first_term} into \eqr{main_equation} and
obtain
$$
  f'^2
  - \bigg(
  \frac{m + 1}{2m}
  \bigg) ff''
  =
  1
  + \frac{m + 1}{2m} f'''
$$
$$
  \bigg(\frac{2m}{m+1}\bigg) f'^2
  - ff''
  =
  \frac{2m}{m+1}
  + f'''
$$
\eqn{result}{
  ff'' 
  + \frac{2m}{1 + m}
  \bigg(1 - f'^2 \bigg)
  + ff''
  =
  0
}
We have the no-slip condition on the edge of the surface,
$$
  f(0) = f'(0) = 0
$$
where $x$ denotes the distance along the surface from the stagnation point, and
$y$ denotes the distance from the surface in the normal direction. We
also have the matching condition
$$
  f'(\infty) = 1
$$
to ensure $u = U$ outside the boundary layer.

If we choose $m = 1$ in \eqr{result}, we obtain the equation derived in the
previous problem for flow past a cylinder. If we choose $m = 0$ we obtain the
equation for flow past a plate in \S 8.3.
\hfill $\blacksquare$
\end{description}
\end{document}
